fixing admits

proof/rejection_sampling/RejectionSampling.ec
@@ -5,6 +5,7 @@ type X.
 abbrev Impl P Q = (forall (x : X), P x => Q x).
 
 op d : X distr.
+op defX : X.                     (* default X *)
 axiom dll : is_lossless d.
 
 
@@ -14,7 +15,7 @@ module RS = {
   proc sample(P : X -> bool,c:int) = {
     var b : bool;
     var x : X;
-    x <- witness;
+    x <- defX;
     b <- false;
     while(!b){
      x <$ d;
