proof/Uniform_distr_extract_ct.ec
@@ -1,5 +1,5 @@
 require import AllCore IntDiv CoreMap List Distr.
-from Jasmin require import JModel.
+require import JModel.
 
 
 
